tests/layeff/LowParseWriters.Sealed.Compat.fst
@@ -13,7 +13,7 @@ let valid_synth_parse_synth'
     LP.synth_injective f2 /\
     LP.synth_inverse f2 f1
   ))
-: Tot (valid_synth_t p1 (parse_synth p1 f2 f1))
+: Tot (squash (valid_synth_prop p1 (parse_synth p1 f2 f1)))
 = tvalid_synth_of_evalid_synth (valid_synth_parse_synth p1 f2 f1 sq)
 
 let valid_synth_parse_synth_recip'
@@ -25,7 +25,7 @@ let valid_synth_parse_synth_recip'
     LP.synth_injective f2 /\
     LP.synth_inverse f2 f1
   ))
-: Tot (valid_synth_t (parse_synth p1 f2 f1) p1)
+: Tot (squash (valid_synth_prop (parse_synth p1 f2 f1) p1))
 = tvalid_synth_of_evalid_synth (valid_synth_parse_synth_recip p1 f2 f1 sq)
 
 module U32 = FStar.UInt32
@@ -43,10 +43,10 @@ let valid_synth_parse_vlarray_intro'
     Parser?.t pa == LP.vlarray (Parser?.t p) elem_count_min elem_count_max /\
     get_parser pa == LP.parse_vlarray (U32.v array_byte_size_min) (U32.v array_byte_size_max) (get_serializer p) elem_count_min elem_count_max ()
   ))
-: Tot (valid_synth_t
+: Tot (squash (valid_synth_prop
     (parse_vllist p array_byte_size_min array_byte_size_max)
     pa
-  )
+  ))
 =
   tvalid_synth_of_evalid_synth (valid_synth_parse_vlarray_intro pa p array_byte_size_min array_byte_size_max elem_count_min elem_count_max u)
 
@@ -63,10 +63,10 @@ let valid_synth_parse_vlarray_elim'
     Parser?.t pa == LP.vlarray (Parser?.t p) elem_count_min elem_count_max /\
     get_parser pa == LP.parse_vlarray (U32.v array_byte_size_min) (U32.v array_byte_size_max) (get_serializer p) elem_count_min elem_count_max ()
   ))
-: Tot (valid_synth_t
+: Tot (squash (valid_synth_prop
     pa
     (parse_vllist p array_byte_size_min array_byte_size_max)
-  )
+  ))
 =
   tvalid_synth_of_evalid_synth (valid_synth_parse_vlarray_elim pa p array_byte_size_min array_byte_size_max elem_count_min elem_count_max u)
 
@@ -82,10 +82,10 @@ let valid_synth_parse_bounded_vldata_intro'
     get_parser_kind pa == LP.parse_bounded_vldata_strong_kind (U32.v min) (U32.v max) (LP.log256' (U32.v max)) (get_parser_kind p) /\
     get_parser pa == LP.parse_bounded_vldata (U32.v min) (U32.v max) (get_parser p)
   })
-: Tot (valid_synth_t
+: Tot (squash (valid_synth_prop
     (parse_vldata p min max)
     pa
-  )
+  ))
 =
   tvalid_synth_of_evalid_synth (valid_synth_parse_bounded_vldata_intro pa p min max)
 
